[mlsexp] Try to make progress in proofs

basis/SexpProgScript.sml
@@ -7,6 +7,7 @@ Ancestors
   ml_translator
   std_prelude  (* OPTION_TYPE *)
   mlbasicsProg  (* Fail_exn *)
+  fsFFIProps  (* forwardFD_o *)
   TextIOProg
   TextIOProof
 Libs
@@ -69,19 +70,19 @@ Quote add_cakeml:
               else raise Fail "lex_aux: missing closing parenthesis"
     | Some c =>
         if Char.isSpace c then lex_aux depth input acc
-        else if c = #"(" then lex_aux (depth + 1) input (OPEN::acc)
+        else if c = #"(" then lex_aux (depth + 1) input (Open::acc)
         else if c = #")" then
           (if depth = 0 then raise Fail "lex_aux: too many closing parenthesis"
-           else if depth = 1 then CLOSE::acc
-           else lex_aux (depth - 1) input (CLOSE::acc))
+           else if depth = 1 then Close::acc
+           else lex_aux (depth - 1) input (Close::acc))
         else if c = #"\"" then
           let val s = read_string input in
-            if depth = 0 then [SYMBOL s]
-            else lex_aux depth input ((SYMBOL s)::acc) end
+            if depth = 0 then [Symbol s]
+            else lex_aux depth input ((Symbol s)::acc) end
         else
           let val s = read_symbol input in
-            if depth = 0 then [SYMBOL s]
-            else lex_aux depth input ((SYMBOL s)::acc) end
+            if depth = 0 then [Symbol s]
+            else lex_aux depth input ((Symbol s)::acc) end
 End
 
 Quote add_cakeml:
@@ -100,63 +101,205 @@ End
 
 val st = get_ml_prog_state ();
 
+Definition read_string_aux_post_def:
+  read_string_aux_post s acc fs is fd =
+    (case read_string_aux s acc of
+     | INL (msg, rest) =>
+         POSTe exn. SEP_EXISTS k.
+           INSTREAM_STR fd is rest (forwardFD fs fd k) *
+           &(Fail_exn msg exn)
+     | INR (slit, rest) =>
+         POSTv slitv. SEP_EXISTS k.
+           STDIO (forwardFD fs fd k) *
+           INSTREAM_STR fd is rest (forwardFD fs fd k) *
+           &(STRING_TYPE slit slitv))
+End
+
+Theorem read_string_aux_spec:
+  ∀s acc accv p is fs fd.
+    LIST_TYPE CHAR acc accv ⇒
+    app (p:'ffi ffi_proj) read_string_aux_v [is; accv]
+      (STDIO fs * INSTREAM_STR fd is s fs)
+      (read_string_aux_post s acc fs is fd)
+Proof
+  Induct
+  \\ rpt strip_tac
+  \\ qmatch_goalsub_abbrev_tac ‘read_string_aux_post s₁’
+  \\ xcf "read_string_aux" st
+  >-
+   (xlet ‘POSTv chv. SEP_EXISTS k.
+             STDIO (forwardFD fs fd k) *
+             INSTREAM_STR fd is (TL s₁) (forwardFD fs fd k) *
+             &OPTION_TYPE CHAR (oHD s₁) chv’
+    >- (xapp_spec b_input1_spec_str)
+    \\ unabbrev_all_tac \\ gvs [OPTION_TYPE_def]
+    \\ xmatch
+    \\ xlet_autop
+    \\ xraise
+    \\ simp [read_string_aux_post_def, read_string_aux_def] \\ xsimpl
+    \\ qexists ‘k’ \\ xsimpl
+    \\ simp [Fail_exn_def])
+  >-
+   (xlet ‘POSTv chv. SEP_EXISTS k.
+             STDIO (forwardFD fs fd k) *
+             INSTREAM_STR fd is (TL s₁) (forwardFD fs fd k) *
+             &OPTION_TYPE CHAR (oHD s₁) chv’
+    >- (xapp_spec b_input1_spec_str)
+    \\ unabbrev_all_tac \\ gvs [OPTION_TYPE_def]
+    \\ xmatch
+    \\ xlet_autop
+    \\ xif
+    >-
+     (xlet_autop
+      \\ xapp \\ xsimpl
+      \\ first_assum $ irule_at (Pos hd)
+      \\ rpt strip_tac
+      \\ simp [read_string_aux_post_def, read_string_aux_def] \\ xsimpl
+      \\ qexists ‘k’ \\ xsimpl)
+    \\ xlet_autop
+    \\ xif
+    >-
+     (rename [‘read_string_aux_post (STRING _ s)’]
+      \\ xlet ‘POSTv chv. SEP_EXISTS k₁.
+                 STDIO (forwardFD fs fd (k + k₁)) *
+                 INSTREAM_STR fd is (TL s) (forwardFD fs fd (k + k₁)) *
+                 &OPTION_TYPE CHAR (oHD s) chv’
+      >-
+       (xapp_spec b_input1_spec_str
+        \\ qexistsl [‘emp’, ‘s’, ‘forwardFD fs fd k’, ‘fd’]
+        \\ simp [forwardFD_o] \\ xsimpl)
+      \\ Cases_on ‘s’ \\ gvs [OPTION_TYPE_def]
+      >-
+       (xmatch \\ xapp
+        \\ first_assum $ irule_at (Pos hd)
+        \\ qexistsl [‘forwardFD fs fd (k + k₁)’, ‘fd’, ‘emp’]
+        \\ conj_tac >- xsimpl
+        \\ simp [read_string_aux_post_def, read_string_aux_def]
+        \\ xsimpl
+        \\ rpt strip_tac \\ simp [forwardFD_o]
+        \\ qmatch_goalsub_abbrev_tac ‘forwardFD fs fd kpx’
+        \\ qexists ‘kpx’ \\ xsimpl)
+      \\ xmatch
+      \\ xlet_autop
+      \\ xif
+      >- cheat
+       (* (xlet_autop *)
+       (*  \\ xapp *)
+       (*  \\ qexistsl [‘emp’, ‘forwardFD fs fd (k + k₁)’, ‘fd’, ‘#"\""::acc’] *)
+       (*  \\ simp [LIST_TYPE_def] *)
+       (*  \\ conj_tac >- (cheat) *)
+       (*  \\ simp [read_string_aux_post_def, read_string_aux_def] *)
+       (*  \\ cheat *)
+         (* ) *)
+      \\ cheat)
+   \\ cheat)
+QED
+
+
+Definition lex_aux_post_def:
+  lex_aux_post depth s acc fs is fd =
+    (case lex_aux depth s acc of
+     | INL (msg, rest) =>
+         POSTe exn. SEP_EXISTS k.
+           INSTREAM_STR fd is rest (forwardFD fs fd k) *
+           &(Fail_exn msg exn)
+     | INR (toks, rest) =>
+         POSTv tokvs. SEP_EXISTS k.
+           STDIO (forwardFD fs fd k) *
+           INSTREAM_STR fd is rest (forwardFD fs fd k) *
+           &(LIST_TYPE MLSEXP_TOKEN_TYPE toks tokvs))
+End
+
+val MLSEXP_TOKEN_TYPE_def = theorem "MLSEXP_TOKEN_TYPE_def";
+
+(* Solve goals of the form
+
+   lex_aux_post ... (forwardFD fs fd k) is fd *+ emp ==+>
+   lex_aux_post ... fs is fd *+ GC
+
+   This usually comes up as part of a recursive call. *)
+val lex_aux_SEP_IMPPOST_tac =
+  (simp [lex_aux_post_def, lex_aux_def, isSpace_def]
+   \\ ntac 2 CASE_TAC
+   \\ simp [forwardFD_o]
+   \\ xsimpl \\ rpt strip_tac
+   \\ qmatch_goalsub_abbrev_tac ‘forwardFD fs fd kpx’
+   \\ qexists ‘kpx’ \\ xsimpl);
+
+(* Finish up the goal when we are returning.
+   Should be preceeded by an x-tactic (xraise, xcon, ...) *)
+val lex_aux_ret_tac =
+  (simp [lex_aux_post_def, lex_aux_def] \\ xsimpl
+   \\ qexists ‘k’ \\ xsimpl
+   \\ simp [LIST_TYPE_def, MLSEXP_TOKEN_TYPE_def, Fail_exn_def]);
+
 Theorem lex_aux_spec:
   ∀s depth depthv acc accv p is fs fd.
     NUM depth depthv ∧ LIST_TYPE MLSEXP_TOKEN_TYPE acc accv ⇒
     app (p:'ffi ffi_proj) lex_aux_v [depthv; is; accv]
       (STDIO fs * INSTREAM_STR fd is s fs)
-      (case lex_aux depth s acc of
-       | INL (msg, rest) =>
-         POSTe exn. SEP_EXISTS k.
-           INSTREAM_STR fd is rest (forwardFD fs fd k) *
-           &(Fail_exn msg exn)
-       | INR (toks, rest) =>
-         POSTv tokvs. SEP_EXISTS k.
-           STDIO (forwardFD fs fd k) *
-           INSTREAM_STR fd is rest (forwardFD fs fd k) *
-           &(LIST_TYPE MLSEXP_TOKEN_TYPE toks tokvs))
+      (lex_aux_post depth s acc fs is fd)
 Proof
-  cheat
-  (* rpt strip_tac *)
-  (* \\ xcf "lex_aux" st *)
-  (* \\ xlet ‘POSTv chv. SEP_EXISTS k. *)
-  (*            STDIO (forwardFD fs fd k) * *)
-  (*            INSTREAM_STR fd is (TL s) (forwardFD fs fd k) * *)
-  (*            &OPTION_TYPE CHAR (oHD s) chv’ *)
-  (* >- (xapp_spec b_input1_spec_str) *)
-  (* \\ Cases_on ‘s’ \\ gvs [OPTION_TYPE_def] *)
-  (* \\ xmatch *)
-  (* >- *)
-  (*  (xlet_auto >- xsimpl *)
-  (*   \\ xif \\ simp [lex_aux_def] *)
-  (*   >- (xvar \\ xsimpl \\ qexists ‘k’ \\ xsimpl) *)
-  (*   \\ xlet_auto >- (xcon \\ xsimpl) *)
-  (*   \\ xraise *)
-  (*   \\ xsimpl \\ qexists ‘k’ \\ xsimpl *)
-  (*   \\ simp [Fail_exn_def]) *)
-  (* \\ xlet_auto >- xsimpl *)
-  (* \\ xif *)
-  (* >- *)
-  (*  (xsimpl *)
-  (*   \\ xapp) *)
-  (* \\ cheat *)
-QED
-
-Theorem lex_spec:
-  app (p:'ffi ffi_proj) lex_v [is]
-    (STDIO fs * INSTREAM_STR fd is s fs)
-    (case lex s of
-     | INL (msg, rest) =>
-       POSTe exn. SEP_EXISTS k.
-         INSTREAM_STR fd is rest (forwardFD fs fd k) *
-         &(Fail_exn msg exn)
-     | INR (toks, rest) =>
-       POSTv tokvs. SEP_EXISTS k.
-         STDIO (forwardFD fs fd k) *
-         INSTREAM_STR fd is rest (forwardFD fs fd k) *
-         &(LIST_TYPE MLSEXP_TOKEN_TYPE toks tokvs))
-Proof
-  xcf "lex" st
-  \\ xlet_auto >- (xcon \\ xsimpl)
-  \\ cheat
+  Induct
+  \\ rpt strip_tac
+  \\ qmatch_goalsub_abbrev_tac ‘lex_aux_post _ s₁’
+  \\ xcf "lex_aux" st
+  >-
+   (xlet ‘POSTv chv. SEP_EXISTS k.
+            STDIO (forwardFD fs fd k) *
+            INSTREAM_STR fd is (TL s₁) (forwardFD fs fd k) *
+            &OPTION_TYPE CHAR (oHD s₁) chv’
+    >- (xapp_spec b_input1_spec_str)
+    \\ unabbrev_all_tac \\ gvs [OPTION_TYPE_def]
+    \\ xmatch
+    \\ xlet_autop
+    \\ xif
+    >-
+     (xvar
+      \\ simp [lex_aux_post_def, lex_aux_def] \\ xsimpl
+      >- (qexists ‘k’ \\ xsimpl))
+    \\ xlet_autop
+    \\ xraise \\ lex_aux_ret_tac)
+  >-
+   (xlet ‘POSTv chv. SEP_EXISTS k.
+            STDIO (forwardFD fs fd k) *
+            INSTREAM_STR fd is (TL s₁) (forwardFD fs fd k) *
+            &OPTION_TYPE CHAR (oHD s₁) chv’
+    >- (xapp_spec b_input1_spec_str)
+    \\ unabbrev_all_tac \\ gvs [OPTION_TYPE_def]
+    \\ xmatch
+    \\ xlet_autop
+    \\ xif >-
+     (last_x_assum $ drule_all_then assume_tac
+      \\ xapp
+      \\ qexistsl [‘emp’, ‘forwardFD fs fd k’, ‘fd’]
+      \\ xpull >- xsimpl
+      \\ lex_aux_SEP_IMPPOST_tac)
+    \\ xlet_autop
+    \\ xif >-
+     (ntac 3 xlet_autop
+      \\ xapp
+      \\ qexistsl [‘emp’, ‘forwardFD fs fd k’, ‘fd’, ‘depth + 1’, ‘OPEN::acc’]
+      \\ simp []
+      \\ conj_tac >- (simp [LIST_TYPE_def, MLSEXP_TOKEN_TYPE_def])
+      \\ xpull >- xsimpl
+      \\ lex_aux_SEP_IMPPOST_tac)
+    \\ xlet_autop
+    \\ xif >-
+     (xlet_autop
+      \\ xif >- (xlet_autop \\ xraise \\ lex_aux_ret_tac)
+      \\ xlet_autop
+      \\ xif >- (xlet_autop \\ xcon \\ lex_aux_ret_tac)
+      \\ ntac 3 xlet_autop
+      \\ xapp
+      \\ qexistsl
+           [‘emp’, ‘forwardFD fs fd k’, ‘fd’, ‘depth - 1’, ‘CLOSE::acc’]
+      \\ simp []
+      \\ conj_tac >- (simp [LIST_TYPE_def, MLSEXP_TOKEN_TYPE_def])
+      \\ xpull >- xsimpl
+      \\ lex_aux_SEP_IMPPOST_tac)
+    \\ xlet_autop
+    \\ xif >-
+     (cheat)
+    \\ cheat)
 QED
